Dafny/examples/BasicBug/simpleBugGeneral.i.dfy
@@ -1,38 +1,73 @@
 include "../../LLVM/llvmREFACTOR.i.dfy"
 include "../../LLVM/types.dfy"
 include "../../Libraries/Seqs.s.dfy"
+include "../../LLVM/behaviorLemmas.i.dfy"
 
 module simpleBugGeneral{
     import opened LLVM_defRE
     import opened types
     import opened Collections__Seqs_s
     import opened Collections__Sets_i
+    import opened behavior_lemmas
 
-        // benignPatch: "The patch does not add any NEW behaviors"
-    predicate benignPatch(a:seq<behavior>,b:seq<behavior>)
+    // benignPatch: "The patch does not add any NEW behaviors"
+    predicate benignPatch(pre:set<behavior>,post:set<behavior>)
     {
-        var aOut := allBehaviorOutput(a);
-        var bOut := allBehaviorOutput(b);
-        forall p :: p in bOut ==> p in aOut
-
+        var preOutput := allBehaviorOutputSet(pre);
+        var postOutput := allBehaviorOutputSet(post);
+        forall postB :: postB in postOutput ==> postB in preOutput
     }
 
   // successfulPatch: "The patch prunes the BAD (defined by MiniSpec) behaviors"
-    predicate successfulPatch(b:seq<behavior>)
+    predicate successfulPatch(post:set<behavior>)
     {
-        forall p :: MiniSpec(p) ==> !(p in b)
+        forall postB :: MiniSpec(postB) ==> !(postB in post)
     }
 
     // completePatch: "The patch preserves the GOOD behavior" // Name; complete -> preserving ? 
-    predicate completePatch(a:seq<behavior>,b:seq<behavior>)
+    predicate completePatch(pre:set<behavior>,post:set<behavior>)
     {
         // forall p :: (p in a && !MiniSpec(p)) ==> p in b
 
-        var aOut := allBehaviorOutput(a);
-        var bOut := allBehaviorOutput(b);
-        forall p :: (behaviorOutput(p) in aOut && !MiniSpec(p)) ==> behaviorOutput(p) in bOut
+        var preOutput := allBehaviorOutputSet(pre);
+        var postOutput := allBehaviorOutputSet(post);
+        forall preB :: (behaviorOutput(preB) in preOutput && !MiniSpec(preB)) ==> behaviorOutput(preB) in postOutput
+    }
+    // completePatch: "The patch preserves the GOOD behavior" // Name; complete -> preserving ? 
+    predicate completePatchMS(pre:set<behavior>,post:set<behavior>)
+    {
+        // forall p :: (p in a && !MiniSpec(p)) ==> p in b
+        var preModMs := MakeSubset(pre, x => !MiniSpec(x));
+        var preModMsOut := allBehaviorOutputSet(preModMs);
+        var postOutput := allBehaviorOutputSet(post);
+        forall preB :: behaviorOutput(preB) in preModMsOut ==> behaviorOutput(preB) in postOutput
     }
 
+
+
+ predicate safePatch(pre:set<behavior>,post:set<behavior>)
+    {
+        // forall p :: (p in a && !MiniSpec(p)) <==> p in b
+        var preOutput := allBehaviorOutputSet(pre);
+        var postOutput := allBehaviorOutputSet(post);
+        forall preB :: (behaviorOutput(preB) in preOutput && !MiniSpec(preB)) <==> behaviorOutput(preB) in postOutput
+    }
+
+    predicate safePatchMS(pre:set<behavior>,post:set<behavior>)
+    {           
+    //  forall p :: (p in a && !MiniSpec(p)) <==> p in b
+        var preModMs := MakeSubset(pre, x => !MiniSpec(x));
+        var preModMsOut := allBehaviorOutputSet(preModMs);
+        var postOutput := allBehaviorOutputSet(post);
+        forall preB :: behaviorOutput(preB) in preModMsOut <==> behaviorOutput(preB) in postOutput
+    }   
+
+
+// lemma fullPatch(a:set<behavior>,b:set<behavior>)
+//     requires benignPatch(a,b);
+//     requires successfulPatch(b);
+//     requires completePatch(a,b);
+//     ensures safePatch(a,b);
 
 // Describes/Excludes 'bad' behaviors in the Unpatched Code (ie preBehaviors)
     predicate RemovedBehaviors(b:behavior)
