Dafny/examples/simpleBenign/simpleBenignisBenign.i.dfy
@@ -1,20 +1,51 @@
 include "BenignCode.s.dfy"
 include "simpleBenignCommon.i.dfy"
-include "../../LLVM/llvmREFACTOR.i.dfy"
+include "../../LLVM/llvmREFACTOR_Multi.i.dfy"
 include "../../LLVM/types.dfy"
 include "../../Libraries/Seqs.s.dfy"
 
 module simpleBenignIsBenign{
     import opened simpleBenignCode
     import opened simpleBenignCommon
-    import opened LLVM_defRE
+    import opened LLVM_defRE_Multi
     import opened types
     import opened Collections__Seqs_s
 
 
-    lemma unwrapPatchSOIBehaviors(s:state, input:operand) returns (b:behavior) 
+lemma unwrapMultiBehaviors(s:state) returns (b:behavior) 
         requires ValidState(s);
         requires SOI_ASSIMPTIONS(s);
+        // ensures exists var_cmp2:operand :: var_cmp2.LV? && var_cmp2.l in s.lvs && var_cmp2.l == "var_cmp2";
+        ensures b == [s] + evalCodeRE(MergedTest(s),s);
+        // ensures ValidBehavior(b);
+        // ensures forall r :: (ValidState(r) && SOI_ASSIMPTIONS(r) && s != r) ==> b == ([s] + evalCodeRE(benign_patch_SOI(r),r))
+    {
+        reveal_ValidBehavior();
+        var var_cmp2 := LV(" var_cmp2 ");
+        var var_0:operand :| var_0.LV? && var_0.l in s.lvs && var_0.l == "var_0";
+    
+        var c := benign_patch_SOI(s);
+        // var if_end := Block([
+        // Ins(ICMP(var_cmp2,ugt,4,var_0,D(Int(0,IntType(4,false))))),
+        // IfElse(true,if_then3().block,if_end4().block)]);
+
+        assert OperandContents(s,var_0).Int?;
+        assert OperandContents(s,var_0).val >= 2147483646;
+
+
+        assert |c.block| == 2;
+
+        b := [s] + evalCodeRE(c,s);
+
+    }
+
+    lemma unwrapPatchSOIBehaviors(s:state) returns (b:behavior) 
+        requires ValidState(s);
+        requires SOI_ASSIMPTIONS(s);
+        // ensures exists var_cmp2:operand :: var_cmp2.LV? && var_cmp2.l in s.lvs && var_cmp2.l == "var_cmp2";
+        ensures b == [s] + evalCodeRE(benign_patch_SOI(s),s);
+        // ensures ValidBehavior(b);
+        // ensures forall r :: (ValidState(r) && SOI_ASSIMPTIONS(r) && s != r) ==> b == ([s] + evalCodeRE(benign_patch_SOI(r),r))
     {
         reveal_ValidBehavior();
         var var_cmp2 := LV(" var_cmp2 ");
@@ -39,12 +70,15 @@ module simpleBenignIsBenign{
 
         assert ValidInstruction(s,ICMP(var_cmp2,ugt,4,var_0,D(Int(0,IntType(4,false)))));
         assert NextStep(b[0],b[1],Step.evalInsStep(ICMP(var_cmp2,ugt,4,var_0,D(Int(0,IntType(4,false))))));
+        // assert OperandContents(b[0],var_0).val > 
         assert StateNext(b[0],b[1]);
 
         assert step == [b[1]];
-        assert remainder == [IfElse(true,if_then3().block,if_end4().block)];
+        assert remainder == [IfElse(var_cmp2,if_then3().block,if_end4().block)];
         assert subBehavior == b[1..];
         assert first(remainder).IfElse?;
+        assert validIfCond(last(step),first(remainder).ifCond);
+        assert dataToBool(OperandContents(last(step),first(remainder).ifCond));
         step,remainder,subBehavior := unwrapBlockWitness(subBehavior,remainder,last(step));
 
         assert step == [b[1]];
@@ -100,8 +134,200 @@ module simpleBenignIsBenign{
         assert remainder == [];
         assert subBehavior == [b[4]] + evalBlockRE(remainder, b[4]);
         assert NextStep(b[4],b[5],Step.stutterStep());
+        // step,remainder,subBehavior := unwrapBlockWitness(subBehavior,remainder,last(step));
+        // assert NextStep(b[5],b[6],Step.stutterStep());
+        //   step,remainder,subBehavior := unwrapBlockWitness(subBehavior,remainder,last(step));
         // assert |b| == 7;
+        assert |b| >  |[b[0],b[1],b[2],b[3],b[4]]|;
+        var simplified := Block([Ins(ICMP(var_cmp2,ugt,4,var_0,D(Int(0,IntType(4,false))))),
+                            Ins(CALL(D(Void),printf_code(global_str()).block)),
+                            Ins(CALL(D(Void),printf_code(global_str1()).block)),
+                            Ins(RET(D(Void)))]);
+
+        assert s == b[0];
+        assert NextStep(b[0],b[1],Step.evalInsStep(ICMP(var_cmp2,ugt,4,var_0,D(Int(0,IntType(4,false))))));
+        assert StateNext(b[0],b[1]);
+        assert NextStep(b[1],b[2],Step.evalInsStep(CALL(D(Void),printf_code(global_str()).block)));
+        assert StateNext(b[1],b[2]); 
+        assert NextStep(b[2],b[3],Step.evalInsStep(CALL(D(Void),printf_code(global_str1()).block)));
+        assert StateNext(b[2],b[3]); 
+        assert NextStep(b[3],b[4],Step.evalInsStep(RET(D(Void))));
+        assert StateNext(b[3],b[4]);
+        assert NextStep(b[4],b[5],Step.stutterStep());
+        assert StateNext(b[4],b[5]);
+        // assert [s] + evalCodeRE(simplified,s) == [b[0],b[1],b[2],b[3],b[4],b[5]];
+
+        // assert evalCodeRE(Block([Ins(ICMP(var_cmp2,ugt,4,var_0,D(Int(0,IntType(4,false)))))]),s)
         assert ValidBehavior(b);
     
     }
+
+    // lemma PatchAlwaysIsCorrect()
+    // {
+    //      forall s:state | ValidState(s) && SOI_ASSIMPTIONS(s)
+    //         // ensures behaviorOutput(postB) == validBehaviorsOuts();
+    //     {
+    //         var b := uunwrapPatchSOIBehaviors(s);
+    //         assert dataToBool(OperandContents(b[1],IfElse(var_cmp2,if_then3().block,if_end4().block).ifCond)); 
+    //     }
+    // }
+
+
+    lemma unwrapVulnSOIBehaviors(s:state) returns (b:behavior) 
+        requires ValidState(s);
+        requires SOI_ASSIMPTIONS(s);
+    {
+        reveal_ValidBehavior();
+        var var_cmp2 := LV(" var_cmp2 ");
+        var var_0:operand :| var_0.LV? && var_0.l in s.lvs && var_0.l == "var_0";
+    
+        var c := benign_vuln_SOI(s);
+        // var if_end := Block([
+        // Ins(ICMP(var_cmp2,ugt,4,var_0,D(Int(0,IntType(4,false))))),
+        // IfElse(true,if_then3().block,if_end4().block)]);
+
+        assert OperandContents(s,var_0).Int?;
+        assert OperandContents(s,var_0).val >= 2147483646;
+
+
+        assert |c.block| == 2;
+
+        b := [s] + evalCodeRE(c,s);
+       
+        var step,remainder,subBehavior := unwrapBlockWitness(b,c.block,s);
+
+        assert b[0] == s;
+
+        assert ValidInstruction(s,ICMP(var_cmp2,sgt,4,var_0,D(Int(0,IntType(4,false)))));
+        assert NextStep(b[0],b[1],Step.evalInsStep(ICMP(var_cmp2,sgt,4,var_0,D(Int(0,IntType(4,false))))));
+        // assert OperandContents(b[0],var_0).val > 
+        assert StateNext(b[0],b[1]);
+
+        assert step == [b[1]];
+        assert remainder == [IfElse(var_cmp2,if_then3().block,if_end4().block)];
+        assert subBehavior == b[1..];
+        assert first(remainder).IfElse?;
+        assert validIfCond(last(step),first(remainder).ifCond);
+        // assert dataToBool(OperandContents(last(step),first(remainder).ifCond));
+        if dataToBool(OperandContents(last(step),first(remainder).ifCond)){ // True Branch
+            step,remainder,subBehavior := unwrapBlockWitness(subBehavior,remainder,last(step));
+
+            assert step == [b[1]];
+            assert remainder == if_then3().block;
+            assert subBehavior == [b[1]] + evalBlockRE(remainder, b[1]); // no state change, just control flow
+
+            assert first(remainder).Ins?;
+            assert first(remainder).ins == CALL(D(Void),printf_code(global_str()).block);
+            step,remainder,subBehavior := unwrapBlockWitness(subBehavior,remainder,last(step));
+            
+            assert step == [b[2]];
+            assert b[2] == evalInsRe(CALL(D(Void),printf_code(global_str()).block),b[1]);
+            unwrapPrintf(b[1],b[2],global_str());
+            assert NextStep(b[1],b[2],Step.evalInsStep(CALL(D(Void),printf_code(global_str()).block)));
+            assert StateNext(b[1],b[2]); 
+            assert remainder == [if_end4()];
+            assert first(remainder).Block?;
+            assert subBehavior == [b[2]] + evalBlockRE(remainder, b[2]);
+
+            
+            step,remainder,subBehavior := unwrapBlockWitness(subBehavior,remainder,last(step));
+            assert step == [b[2]];
+            assert remainder == if_end4().block;
+            assert subBehavior == [b[2]] + evalBlockRE(remainder, b[2]); // no state change, just control flow
+
+            assert first(remainder).Ins?;
+            assert first(remainder).ins == CALL(D(Void),printf_code(global_str1()).block);
+
+            step,remainder,subBehavior := unwrapBlockWitness(subBehavior,remainder,last(step));
+            assert step == [b[3]];
+            assert b[3] == evalInsRe(CALL(D(Void),printf_code(global_str1()).block),b[2]);
+            unwrapPrintf(b[2],b[3],global_str1());
+            assert NextStep(b[2],b[3],Step.evalInsStep(CALL(D(Void),printf_code(global_str1()).block)));
+            assert StateNext(b[2],b[3]); 
+            assert remainder == [return_()];
+            assert first(remainder).Block?;
+            assert subBehavior == [b[3]] + evalBlockRE(remainder, b[3]);
+
+            step,remainder,subBehavior := unwrapBlockWitness(subBehavior,remainder,last(step));
+            assert step == [b[3]];
+            assert remainder == return_().block;
+            assert subBehavior == [b[3]] + evalBlockRE(remainder, b[3]);// no state change, just control flow
+
+            assert first(remainder).Ins?;
+            assert first(remainder).ins == RET(D(Void));
+            step,remainder,subBehavior := unwrapBlockWitness(subBehavior,remainder,last(step));
+            assert step == [b[4]];
+            assert b[4] == evalInsRe(RET(D(Void)),b[3]);
+            assert NextStep(b[3],b[4],Step.evalInsStep(RET(D(Void))));
+            assert StateNext(b[3],b[4]);
+
+            assert remainder == [];
+            assert subBehavior == [b[4]] + evalBlockRE(remainder, b[4]);
+            assert NextStep(b[4],b[5],Step.stutterStep());
+            assert ValidBehavior(b);
+        }else{ //FALSE BRANCH
+            step,remainder,subBehavior := unwrapBlockWitness(subBehavior,remainder,last(step));
+
+            assert step == [b[1]];
+            assert remainder == if_end4().block;
+            assert subBehavior == [b[1]] + evalBlockRE(remainder, b[1]); // no state change, just control flow
+            assert first(remainder).Ins?;
+            assert first(remainder).ins == CALL(D(Void),printf_code(global_str1()).block);
+
+            step,remainder,subBehavior := unwrapBlockWitness(subBehavior,remainder,last(step));
+            assert step == [b[2]];
+            assert b[2] == evalInsRe(CALL(D(Void),printf_code(global_str1()).block),b[1]);
+            unwrapPrintf(b[1],b[2],global_str1());
+            assert NextStep(b[1],b[2],Step.evalInsStep(CALL(D(Void),printf_code(global_str1()).block)));
+            assert StateNext(b[1],b[2]); 
+            assert remainder == [return_()];
+            assert first(remainder).Block?;
+            assert subBehavior == [b[2]] + evalBlockRE(remainder, b[2]);
+
+            step,remainder,subBehavior := unwrapBlockWitness(subBehavior,remainder,last(step));
+            assert step == [b[2]];
+            assert remainder == return_().block;
+            assert subBehavior == [b[2]] + evalBlockRE(remainder, b[2]);// no state change, just control flow
+
+            assert first(remainder).Ins?;
+            assert first(remainder).ins == RET(D(Void));
+            step,remainder,subBehavior := unwrapBlockWitness(subBehavior,remainder,last(step));
+            assert step == [b[3]];
+            assert b[3] == evalInsRe(RET(D(Void)),b[2]);
+            assert NextStep(b[2],b[3],Step.evalInsStep(RET(D(Void))));
+            assert StateNext(b[2],b[3]);
+
+            assert remainder == [];
+            assert subBehavior == [b[3]] + evalBlockRE(remainder, b[3]);
+            assert NextStep(b[3],b[4],Step.stutterStep());
+            assert ValidBehavior(b);
+            
+        }
+       
+    
+    }
+
+    // lemma PatchAlwaysIsCorrect()
+    // {
+    //     forall s,r | ValidState(s) && SOI_ASSIMPTIONS(s) && ValidState(r) && SOI_ASSIMPTIONS(r) 
+    //         // ensures behaviorOutput(postB) == validBehaviorsOuts();
+    //     {
+    //         var b_patch := unwrapPatchSOIBehaviors(s);
+    //         var b_vuln := unwrapPatchSOIBehaviors(r);
+
+    //         // assert b_patch == b_vuln;
+    //     }
+
+
+    //      forall s:state | ValidState(s) && SOI_ASSIMPTIONS(s) && s.lvs["var_0"].val == 2147483646
+    //         // ensures behaviorOutput(postB) == validBehaviorsOuts();
+    //     {
+    //         var b_patch := unwrapPatchSOIBehaviors(s);
+    //         var b_vuln := unwrapVulnSOIBehaviors(s);
+
+    //         assert b_patch == b_vuln;
+    //     }
+    // }
+
+
 }
